@prefix dc:      <http://purl.org/dc/elements/1.1/> .
@prefix app:     <http://jmvanel.free.fr/ontology/software_applications.owl#> .
@prefix list:    <http://www.w3.org/2000/10/swap/list#> .
@prefix log:     <http://www.w3.org/2000/10/swap/log#> .
@prefix grddl:   <http://www.w3.org/2003/g/data-view#> .
@prefix rdfs:    <http://www.w3.org/2000/01/rdf-schema#> .
@prefix owl:     <http://www.w3.org/2002/07/owl#> .
@prefix xsd:     <http://www.w3.org/2001/XMLSchema#> .
@prefix dbpedia:  <http://dbpedia.org/resource/> .
@prefix rdf:     <http://www.w3.org/1999/02/22-rdf-syntax-ns#> .
@prefix doas:    <file:///home/ubuntu/temp/ahmad88me@gmail.com/#> .
@prefix doap:    <http://usefulinc.com/ns/doap#> .

doas:modelingTechnology
      a       owl:ObjectProperty ;
      rdfs:comment "modeling technology, as dbPdedia URI's; e.g. OWL, UML, SQL, Swagger, ..."@en ;
      rdfs:domain doas:Software ;
      rdfs:label "modeling technology"@en ;
      rdfs:range owl:Thing .

doas:inputFileTypes
      a       owl:ObjectProperty ;
      rdfs:comment "input file types, as dbPdedia URI's"@en ;
      rdfs:domain doas:Software ;
      rdfs:label "input file types"@en ;
      rdfs:range owl:Thing .

doas:features
      a       owl:ObjectProperty ;
      rdfs:comment "features, as dbPdedia URI's"@en ;
      rdfs:domain doas:Software ;
      rdfs:label "features"@en ;
      rdfs:range owl:Thing .

doas:uiTechnology
      a       owl:ObjectProperty ;
      rdfs:comment "User interface, a broad platform or library name, like web browser, Java Swing, TCL/TK, as dbPdedia URI's"@en ;
      rdfs:domain doas:Software ;
      rdfs:label "UI"@en ;
      rdfs:range owl:Thing .

doas:isPluginOf
      a       owl:ObjectProperty ;
      rdfs:comment "embedding software if this sowftware is a plugin or module, as dbPdedia URI's; e.g. Firefox, Chrome, Apache, Protégé, ..."@en ;
      rdfs:domain doas:Software ;
      rdfs:label "plugin of"@en ;
      rdfs:range doas:Software .

doas:
      a       owl:Ontology ;
      rdfs:comment """Description Of A Software, a formal Description of a software focusing on architecture, feature, and input/output, enabling to search a software component according to needs,
and leveraging on dbPdedia.
complementary to DOAP."""@en ;
      rdfs:label "Description Of A Software" .

doas:language
      a       owl:ObjectProperty ;
      rdfs:comment "programming language, as dbPdedia URI's"@en ;
      rdfs:domain doas:Software ;
      rdfs:label "language"@en ;
      rdfs:range owl:Thing .

doas:Software
      a       owl:Class ;
      rdfs:label "A software"@en ;
      rdfs:subclassOf doap:Project .

doas:dependencyManager
      a       owl:ObjectProperty ;
      rdfs:comment "dependency Manager like npm, Maven, SBT, or explicitely dbpedia:Nothing, as dbPdedia URI's"@en ;
      rdfs:domain doas:Software ;
      rdfs:label "dependency Manager"@en ;
      rdfs:range owl:Thing .

doas:outputFileTypes
      a       owl:ObjectProperty ;
      rdfs:comment "output file types, as dbPdedia URI's"@en ;
      rdfs:domain doas:Software ;
      rdfs:label "output file types"@en ;
      rdfs:range owl:Thing .

doas:hasProject
      a       owl:ObjectProperty ;
      rdfs:comment "the associated project(s)"@en ;
      rdfs:domain doas:Software ;
      rdfs:label "project"@en ;
      rdfs:range doap:Project .

doas:softwareType
      a       owl:ObjectProperty ;
      rdfs:comment "software type : client, server, library, compiler, etc (as dbPdedia URI)"@en ;
      rdfs:domain doas:Software ;
      rdfs:label "software type"@en ;
      rdfs:range owl:Thing .
